More WIP: fast proof of path replacement

theories/Dot/syn/pathrepl.v
@@ -4,12 +4,112 @@ From D.Dot.syn Require Import syn.
 From D.Dot.lr Require Import unary_lr.
 
 Implicit Types
-         (T : ty) (v : vl) (t : tm) (d : dm) (ds : dms) (p q : path)
+         (T : ty) (v w : vl) (t : tm) (d : dm) (ds : dms) (p q : path)
          (Γ : ctx) (vs : vls) (l : label).
 
+Implicit Types (Pv : vl → Prop).
 Set Nested Proofs Allowed.
 
-Lemma ren_scons v ρ : ren (+1) >> v .: ρ = ρ. Proof. done. Qed.
+(* XXX For Iris *)
+Hint Extern 1 (environments.envs_entails _ (_ ∗-∗ _)) => iSplit : core.
+
+Lemma ren_scons v ρ : ren (+1) >> v .: ρ = ρ.
+Proof. done. Qed.
+
+Fixpoint path_wp_pure p Pv : Prop :=
+  match p with
+  | pself p l => path_wp_pure p (λ v, ∃ w, v @ l ↘ dvl w ∧ Pv w)
+  | pv vp => Pv vp
+  end.
+
+Global Instance Proper_pwp: Proper ((=) ==> pointwise_relation _ iff ==> iff) path_wp_pure.
+Proof.
+  (* The induction works best in this shape, but this instance is best kept local. *)
+  have Proper_pwp_2: ∀ p, Proper (pointwise_relation _ iff ==> iff) (path_wp_pure p).
+  elim; solve_proper.
+  solve_proper.
+Qed.
+
+Lemma path_wp_pure_wand {Pv1 Pv2 p}:
+  path_wp_pure p Pv1 →
+  (∀ v, Pv1 v → Pv2 v) →
+  path_wp_pure p Pv2.
+Proof.
+  elim: p Pv1 Pv2 => /= [v|p IHp l] Pv1 Pv2 Hp Hwand;
+    first by apply Hwand.
+  apply: (IHp _ _ Hp) => {IHp Hp} v [vq [??]].
+  eauto.
+Qed.
+
+Lemma path_wp_pure_eq p Pv :
+  path_wp_pure p Pv ↔ ∃ v, path_wp_pure p (λ w, w = v) ∧ Pv v.
+Proof.
+  elim: p Pv => [ v | p IHp l ] Pv /=; split.
+  - eauto.
+  - by destruct 1 as (w & <- & ?).
+  - rewrite IHp.
+    destruct 1 as (v & Hp & w & ?&?).
+    eexists w; split; last by [].
+    apply (path_wp_pure_wand Hp).
+    intros; subst; exists w; eauto.
+  - setoid_rewrite IHp; intros; ev; subst; eauto.
+Qed.
+
+Lemma path_wp_pure_det {p v1 v2}:
+  path_wp_pure p (λ w, w = v1) →
+  path_wp_pure p (λ w, w = v2) →
+  v1 = v2.
+Proof.
+  elim: p v1 v2 => [v /=| p /= IHp l //] v1 v2;
+    first by intros <- <-.
+  rewrite !path_wp_pure_eq.
+  destruct 1 as (w1 & Hp1 & ?); destruct 1 as (w2 & Hp2 & ?); ev; simplify_eq.
+  pose proof (IHp _ _ Hp1 Hp2) as <-.
+  by objLookupDet.
+Qed.
+
+Lemma path_wp_pure_swap p u :
+  path_wp_pure p (λ w, u = w) ↔
+  path_wp_pure p (λ w, w = u).
+Proof. split => Hp; exact: path_wp_pure_wand. Qed.
+
+Definition alias_paths_pure p q ρ :=
+  path_wp_pure p.|[ρ] (λ vp, path_wp_pure q.|[ρ] (λ vq, vp = vq)).
+
+Lemma alias_paths_pure_refl_vl v ρ :
+  alias_paths_pure (pv v) (pv v) ρ.
+Proof. done. Qed.
+
+Lemma alias_paths_pure_eq p q ρ:
+  alias_paths_pure p q ρ ↔
+  ∃ v,
+    path_wp_pure p.|[ρ] (λ vp, vp = v) ∧
+    path_wp_pure q.|[ρ] (λ vq, vq = v).
+Proof.
+  rewrite /= /alias_paths_pure !path_wp_pure_eq. split => -[vp];
+    [ rewrite (path_wp_pure_swap q.|[_]) |
+      rewrite -(path_wp_pure_swap q.|[_]) ]; eauto.
+Qed.
+
+Lemma alias_paths_pure_symm p q ρ :
+  alias_paths_pure p q ρ → alias_paths_pure q p ρ.
+Proof. rewrite !alias_paths_pure_eq. intros; ev; eauto. Qed.
+
+Lemma alias_paths_equiv_pure p q ρ:
+  alias_paths_pure p q ρ ↔
+    (∃ u, path_wp_pure p.|[ρ] (λ vp, vp = u)) ∧
+    ∀ Pv, path_wp_pure p.|[ρ] Pv ↔ path_wp_pure q.|[ρ] Pv.
+Proof.
+  rewrite alias_paths_pure_eq; split.
+  - destruct 1 as (v & Hp & Hq).
+    split. by eauto. intros Pv.
+    rewrite !path_wp_pure_eq.
+    f_equiv => w; split => -[Hr];
+      [ rewrite -(path_wp_pure_det Hp Hr)
+      | rewrite -(path_wp_pure_det Hq Hr)]; auto.
+  - intros [[u Hp] Heq]. exists u.
+    split; by [|rewrite -Heq].
+Qed.
 
 Section equivI_utils.
   Context `{dlangG Σ}.
@@ -140,17 +240,45 @@ where "T1 ~p[ p := q  ] T2" := (ty_path_repl p q T1 T2) .
 Lemma ty_path_repl_id p T1 T2 : T1 ~p[ p := p ] T2 → T1 = T2.
 Proof. intros Hr; dependent induction Hr; by rewrite // ?IHHr // psubst_path_id. Qed.
 
-Section foo.
+Section path_repl.
   Context `{dlangG Σ}.
   Implicit Types (φ: vl → iProp Σ).
+
+  Lemma path_wp_pureable p Pv:
+    path_wp p (λ v, ⌜Pv v⌝) ⊣⊢@{iPropI Σ} ⌜path_wp_pure p Pv⌝.
+  Proof.
+    elim: p Pv => /= [//|p IHp l] Pv.
+    by rewrite -{}IHp; f_equiv => v; iIntros "!% /=".
+  Qed.
+
+  Global Instance path_wp_pureableI p Pv :
+   IntoPure (@path_wp Σ p (λ v, ⌜Pv v⌝))%I (path_wp_pure p Pv).
+  Proof. by rewrite /IntoPure path_wp_pureable. Qed.
+  Global Instance path_wp_pureableF p Pv :
+   FromPure false  (@path_wp Σ p (λ v, ⌜Pv v⌝))%I (path_wp_pure p Pv).
+  Proof. by rewrite /FromPure/= path_wp_pureable. Qed.
 
   Lemma path_wp_swap p u :
     path_wp p (λ w, ⌜u = w⌝) ⊣⊢@{iPropI Σ}
     path_wp p (λ w, ⌜w = u⌝).
-  Proof. iSplit; iIntros "H"; iApply (path_wp_wand with "H"); auto. Qed.
+  Proof. iIntros "!%". by rewrite /= path_wp_pure_swap. Qed.
 
   Definition alias_paths p q ρ : iProp Σ :=
     path_wp p.|[ρ] (λ vp, path_wp q.|[ρ] (λ vq, ⌜vp = vq⌝))%I.
+
+  Lemma alias_paths_pureable p q ρ:
+    alias_paths p q ρ ⊣⊢ ⌜alias_paths_pure p q ρ⌝.
+  Proof.
+    rewrite /alias_paths/= -path_wp_pureable.
+    f_equiv => vp. apply path_wp_pureable.
+  Qed.
+
+  Global Instance alias_paths_pureableI p q ρ :
+   IntoPure (alias_paths p q ρ) (alias_paths_pure p q ρ).
+  Proof. by rewrite /IntoPure alias_paths_pureable. Qed.
+  Global Instance alias_paths_pureableF p q ρ :
+   FromPure false (alias_paths p q ρ) (alias_paths_pure p q ρ).
+  Proof. by rewrite /FromPure/= alias_paths_pureable. Qed.
 
   Lemma alias_paths_refl_vl v ρ :
     alias_paths (pv v) (pv v) ρ.
@@ -161,15 +289,14 @@ Section foo.
     ∃ v,
       path_wp p.|[ρ] (λ vp : vl, ⌜vp = v⌝) ∧
       path_wp q.|[ρ] (λ vq : vl, ⌜vq = v⌝).
-  Proof.
-    rewrite /= /alias_paths !path_wp_eq; iSplit; iDestruct 1 as (vp) "[Hp Hq]".
-    rewrite (path_wp_swap q.|[_]). eauto.
-    rewrite -(path_wp_swap q.|[_]). eauto.
-  Qed.
+  Proof. iIntros "!%"; rewrite /= alias_paths_pure_eq. intuition. Qed.
 
   Lemma alias_paths_symm p q ρ :
     alias_paths p q ρ -∗ alias_paths q p ρ.
-  Proof. rewrite !alias_paths_eq. iDestruct 1 as (vp) "[Hp Hq]". eauto. Qed.
+  Proof.
+    rewrite !alias_paths_pureable; iIntros "!%".
+    exact: alias_paths_pure_symm.
+  Qed.
 
   Lemma simpl_alias_1 p vr ρ :
      alias_paths p (pv vr) ρ ⊣⊢ path_wp p.|[ρ] (λ w : vl, ⌜w = vr.[ρ]⌝) .
@@ -179,55 +306,76 @@ Section foo.
      alias_paths (pv vr) p ρ ⊣⊢ path_wp p.|[ρ] (λ w : vl, ⌜w = vr.[ρ]⌝) .
   Proof. exact: path_wp_swap. Qed.
 
+  Ltac iProperness :=
+    repeat first
+    [ iEval (progress rewrite -(wp_equivI, exists_equivI, forall_equivI)); iIntros
+    (* f_equiv must come before those others for performance. *)
+    | iEval (progress rewrite -(f_equiv, and2_equivI, wand2_equivI, or2_equivI))
+    ].
+
+  (* Not provable through pure props for impure [φ]. *)
   Lemma alias_paths_equiv p q ρ:
-    alias_paths p q ρ ⊣⊢
-    (∃ u, path_wp p.|[ρ] (λ vp : vl, ⌜vp = u⌝)) ∧ ∀ φ, path_wp p.|[ρ] φ ≡ path_wp q.|[ρ] φ.
+    alias_paths_pure p q ρ ↔
+      (∃ u, path_wp_pure p.|[ρ] (λ vp, vp = u)) ∧
+      ∀ φ, path_wp p.|[ρ] φ ≡ path_wp q.|[ρ] φ.
   Proof.
-    rewrite alias_paths_eq; iSplit.
-    - iDestruct 1 as (v) "#[Hp Hq]".
-      iSplit; first by [auto]; iIntros (φ).
-      iEval (rewrite !path_wp_eq -exists_equivI); iIntros (w).
-      iApply prop_ext; iModIntro; iSplit; iIntros "[H $]";
-        [ iDestruct (path_wp_det with "Hp H") as %<- |
-          iDestruct (path_wp_det with "Hq H") as %<- ]; iFrame "#".
-    - iIntros "[Hterm Heq]". iDestruct "Hterm" as (u) "#Hp". iExists u.
-      iFrame "Hp".
-      by iRewrite -("Heq" $! (λ vp : vl, ⌜vp = u⌝))%I.
+    rewrite alias_paths_pure_eq; split.
+    - destruct 1 as (v & Hp & Hq).
+      split; first by [eauto]; intros φ.
+      rewrite !path_wp_eq. f_equiv => w.
+      rewrite !path_wp_pureable; do 2 f_equiv.
+      split => Hr; [ rewrite -(path_wp_pure_det Hp Hr)
+        | rewrite -(path_wp_pure_det Hq Hr)]; auto.
+    - destruct 1 as ((u & Hp) & Heq). exists u; split; first done.
+      (* Yes, completely insane. *)
+      apply (pure_soundness (M := iResUR Σ)).
+      iRevert (Hp). by rewrite -!path_wp_pureable Heq.
   Qed.
+
+  Lemma alias_paths_equiv' p q ρ:
+    ⌜alias_paths_pure p q ρ⌝ ⊣⊢@{iPropI Σ}
+      (∃ u, path_wp p.|[ρ] (λ vp, ⌜vp = u⌝)) ∧
+      ∀ φ, ⌜path_wp p.|[ρ] φ ≡ path_wp q.|[ρ] φ⌝.
+  Proof. iIntros "!%". apply alias_paths_equiv. Qed.
 
   Lemma alias_paths_elim_eq φ p q ρ:
-    alias_paths p q ρ -∗
+    alias_paths_pure p q ρ →
     path_wp p.|[ρ] φ ≡ path_wp q.|[ρ] φ.
-  Proof. rewrite alias_paths_equiv. iDestruct 1 as "[_ Heq]". iApply "Heq". Qed.
+  Proof. intros ?%alias_paths_equiv. intuition. Qed.
+
+  Lemma alias_paths_elim_eq' φ p q ρ:
+    ⌜alias_paths_pure p q ρ⌝ ⊢@{iPropI Σ}
+    ⌜path_wp p.|[ρ] φ ≡ path_wp q.|[ρ] φ⌝.
+  Proof. iIntros "!%". apply alias_paths_elim_eq. Qed.
 
   Lemma alias_paths_elim_wand p q ρ φ:
-    alias_paths p q ρ -∗
+    ⌜alias_paths_pure p q ρ⌝ ⊢@{iPropI Σ}
     path_wp p.|[ρ] φ -∗ path_wp q.|[ρ] φ.
-  Proof.
-    rewrite (alias_paths_elim_eq φ). iIntros "Heq"; iRewrite "Heq"; auto.
-  Qed.
+  Proof. rewrite (alias_paths_elim_eq' φ). iIntros (->) "$". Qed.
 
   Lemma path_replacement_equiv_plain {p r ρ} q (φ : vl → iProp Σ):
-    alias_paths p r ρ ⊢@{iPropI Σ}
+    alias_paths_pure p r ρ →
     path_wp q.|[ρ] φ ≡ path_wp (q .p[p := r]).|[ρ] φ.
   Proof.
-    elim: q φ => [w | q IHq l] φ /=;
-     case_decide; simplify_eq/=.
+    elim: q φ => [w | q IHq l] φ /=; case_decide; simplify_eq/=.
     - apply (alias_paths_elim_eq φ (pv w) r).
-    - by iIntros.
-    - rewrite /= !path_wp_eq alias_paths_eq /=.
-      iDestruct 1 as (vr) "[Hq' #Hr]".
-      iDestruct (path_wp_eq with "Hq'") as (vq) "#[Hq A]";
-        iDestruct "A" as %(? & Hl & ->).
-      iApply prop_ext; iModIntro; iSplit.
-      + iDestruct 1 as (vq') "[Hq' A]"; iDestruct "A" as (vr' Hl') "Hφ".
-        iDestruct (path_wp_det with "Hq Hq'") as %<-; iClear "Hq Hq'".
-        by objLookupDet; eauto.
-      + iDestruct 1 as (vr') "[Hr' Hφ]".
-        iDestruct (path_wp_det with "Hr Hr'") as %<-; iClear "Hr'".
+    - done.
+    - rewrite /= !path_wp_eq alias_paths_pure_eq /=.
+      destruct 1 as (vr & (vq & Hq & w & Hl & ->)%path_wp_pure_eq & Hr).
+      iSplit.
+      + iDestruct 1 as (vq' Hq' vr' Hl') "Hφ".
+        rewrite (path_wp_pure_det Hq' Hq) in Hl'.
+        objLookupDet. eauto.
+      + iDestruct 1 as (vr' Hr') "Hφ".
+        rewrite (path_wp_pure_det Hr' Hr).
         eauto.
-    - iIntros. by iApply IHq.
+    - exact: IHq.
   Qed.
+
+  Lemma path_replacement_equiv_plain' {p r ρ} q (φ : vl → iProp Σ):
+    ⌜alias_paths_pure p r ρ⌝ ⊢@{iPropI Σ}
+    path_wp q.|[ρ] φ ≡ path_wp (q .p[p := r]).|[ρ] φ.
+  Proof. iIntros (?) "!%". exact: path_replacement_equiv_plain. Qed.
 
   (* Lemma path_replacement_equiv_pure {p r ρ} q (φ : vl → iProp Σ):
     alias_paths p r ρ ⊢@{iPropI Σ}
@@ -258,9 +406,9 @@ Section foo.
   Proof. rewrite path_replacement_equiv_pure. by iIntros (<-). Qed. *)
 
   Lemma rewrite_tsel_psubst2 p q l ρ v r:
-    alias_paths p r ρ ⊢@{iPropI Σ}
+    ⌜alias_paths_pure p r ρ⌝ ⊢@{iPropI Σ}
     ⟦ TSel q l ⟧ ρ v ≡ ⟦ TSel (q .p[ p := r ]) l ⟧ ρ v.
-  Proof. exact: path_replacement_equiv_plain. Qed.
+  Proof. exact: path_replacement_equiv_plain'. Qed.
 
   (* That's false. *)
   (* Lemma path_replacement_equiv_0 {p r ρ} q:
@@ -277,86 +425,48 @@ Section foo.
   Abort. *)
 
   Lemma path_replacement_equiv p q r ρ (φ : vl → iProp Σ):
-    □alias_paths p r ρ ⊢@{iPropI Σ}
+    ⌜alias_paths_pure p r ρ⌝ ⊢@{iPropI Σ}
     □(path_wp q.|[ρ] φ ∗-∗ path_wp (q .p[p := r]).|[ρ] φ).
   Proof.
     iIntros "#H !>".
-    iRewrite -(path_replacement_equiv_plain q φ with "H").
+    iRewrite -(path_replacement_equiv_plain' q φ with "H").
     by rewrite -wand_iff_refl.
   Qed.
 
-  Global Instance Proper_pwp: Proper ((=) ==> pointwise_relation _ (≡) ==> (≡)) (@path_wp Σ).
+  Lemma alias_path_pure_weaken p q ρ v:
+     alias_paths_pure p.|[ren (+1)] q.|[ren (+1)] (v .: ρ) ↔
+     alias_paths_pure p q ρ.
   Proof.
-    (* The induction works best in this shape, but this instance is best kept local. *)
-    have Proper_pwp_2: ∀ p, Proper (pointwise_relation _ (≡) ==> (≡)) (@path_wp Σ p).
-    elim; solve_proper.
-    solve_proper.
+    by rewrite /alias_paths_pure; f_equiv; rewrite hsubst_comp ren_scons.
   Qed.
-
-  Lemma alias_path_weaken p q ρ v:
-     alias_paths p.|[ren (+1)] q.|[ren (+1)] (v .: ρ) ≡ alias_paths p q ρ.
-  Proof. by rewrite /alias_paths; f_equiv; rewrite hsubst_comp ren_scons. Qed.
-
-  (* Ltac iProperness :=
-    repeat first
-    [ rewrite -!f_equiv
-    | rewrite -exists_equivI; iIntros
-    | rewrite -forall_equivI; iIntros
-    | rewrite -wp_equivI; iIntros
-    | progress rewrite -?and2_equivI -?wand2_equivI -?or2_equivI
-    ]. *)
-
-  Ltac iProperness :=
-    repeat first
-    [ iEval (progress rewrite -(wp_equivI, exists_equivI, forall_equivI)); iIntros
-    (* f_equiv must come before those others for performance. *)
-    | iEval (progress rewrite -(f_equiv, and2_equivI, wand2_equivI, or2_equivI))
-    ].
-
-  (* XXX interesting because using properness seems so much faster. *)
-  (* Lemma rewrite_ty_path_repl_plain p q T1 T2 ρ v:
-    T1 ~p[ p := q ] T2 →
-    alias_paths p q ρ →
-    ⟦ T1 ⟧ ρ v ≡ ⟦ T2 ⟧ ρ v.
-  Proof.
-    move => Hrew; move: v ρ.
-    Time induction Hrew => v ρ He /=; properness;
-      try by [|iApply IHHrew; rewrite ?alias_path_weaken].
-    iApply (path_replacement_equiv_plain).
-  Time Qed. *)
-
-  Ltac iProperness ::=
-    repeat first
-    [ iEval (progress rewrite -(wp_equivI, exists_equivI, forall_equivI)); iIntros
-    (* f_equiv must come before those others for performance. *)
-    | iEval (progress rewrite -(f_equiv, and2_equivI, wand2_equivI, or2_equivI))
-    ].
-
-  (* Lemma rewrite_ty_path_repl_plain_weird p q T1 T2 ρ v:
-    T1 ~p[ p := q ] T2 →
-    alias_paths p q ρ →
-    (⟦ T1 ⟧ ρ v ≡ ⟦ T2 ⟧ ρ v : iProp Σ)%I.
-  Proof.
-    move => Hrew; move: v ρ.
-    Time induction Hrew => v ρ He /=; last (iApply path_replacement_equiv_plain; iApply He);
-     iProperness => //; by [iApply IHHrew; rewrite ?alias_path_weaken].
-  Time Qed. *)
 
   Lemma rewrite_ty_path_repl_plain p q T1 T2 ρ v:
     T1 ~p[ p := q ] T2 →
-    alias_paths p q ρ ⊢@{iPropI Σ} (* p : q.type *)
+    alias_paths_pure p q ρ →
     ⟦ T1 ⟧ ρ v ≡ ⟦ T2 ⟧ ρ v.
   Proof.
-    (* move => Hrew. *)
-    (* Time iInduction Hrew as [] "IHHrew" forall (v ρ); last iApply path_replacement_equiv_plain;
-      iIntros "/= #H"; iProperness;
-      try by [iApply "IHHrew"; rewrite ?alias_path_weaken].
-  Time Qed. *)
     move => Hrew; move: v ρ.
-    induction Hrew => v ρ; last apply path_replacement_equiv_plain;
-      iIntros "/= #H"; iProperness;
-      try by [iApply IHHrew; rewrite ?alias_path_weaken].
+    induction Hrew => v ρ He /=; properness;
+      by [|exact: path_replacement_equiv_plain|iApply IHHrew; rewrite ?alias_path_pure_weaken].
   Qed.
+
+  Lemma rewrite_ty_path_repl_plain' p q T1 T2 ρ v:
+    T1 ~p[ p := q ] T2 →
+    alias_paths p q ρ ⊢@{iPropI Σ} (* p : q.type *)
+    ⟦ T1 ⟧ ρ v ≡ ⟦ T2 ⟧ ρ v.
+  Proof. iIntros "!% /=". exact: rewrite_ty_path_repl_plain. Qed.
+
+  (* Lemma rewrite_ty_path_repl_plain'_slow p q T1 T2 ρ v:
+    T1 ~p[ p := q ] T2 →
+    ⌜alias_paths_pure p q ρ⌝ ⊢@{iPropI Σ} (* p : q.type *)
+    ⟦ T1 ⟧ ρ v ≡ ⟦ T2 ⟧ ρ v.
+  Proof.
+    move => Hrew; move: v ρ.
+    induction Hrew => v ρ;
+      iIntros "/= #H"; iProperness; last
+      iApply path_replacement_equiv_plain';
+      try by [|iApply IHHrew; rewrite ?alias_path_pure_weaken].
+  Qed. *)
 
   (* Lemma TMu_E Γ T v: Γ ⊨ tv v : TMu T -∗ Γ ⊨ tv v : T.|[ids 0/] .p [.
   Proof. by rewrite TMu_equiv. Qed.
@@ -394,16 +504,29 @@ Section foo.
       try by iRewrite ("IHHrew" with "[//] H").
        iApply prop_ext; iModIntro; iSplit. *)
 
+(* Axiom skip: forall a, a. *)
+  (* Special cases, any use? *)
+  (* Lemma path_replacement_equiv_plain_special {p vr ρ} q (φ : vl → iProp Σ):
+    path_wp p.|[ρ] (λ w, ⌜ w = vr.[ρ] ⌝) ⊢@{iPropI Σ}
+    path_wp q.|[ρ] φ ≡ path_wp (q .p[p := pv vr]).|[ρ] φ.
+  Proof. rewrite -path_replacement_equiv_plain' -simpl_alias_1.
+  by iIntros "!%". Qed.
+
+  Lemma rewrite_tsel_psubst2_special p q l ρ v vr:
+    path_wp p.|[ρ] (λ w, ⌜ w = vr.[ρ] ⌝) ⊢@{iPropI Σ}
+    ⟦ TSel q l ⟧ ρ v ≡ ⟦ TSel (q .p[ p := pv vr ]) l ⟧ ρ v.
+  Proof. exact: path_replacement_equiv_plain_special. Qed. *)
+
   (* Lemma rewrite_ty_path_repl p T1 T2 ρ v vr:
     T1 ~p[ p := pv vr ] T2 →
-    path_wp p.|[ρ] (λ w, ⌜ w = vr.[ρ] ⌝) -∗ (* p : vr.type *)
-    (⟦ T1 ⟧ ρ v ∗-∗ ⟦ T2 ⟧ ρ v).
+    path_wp p.|[ρ] (λ w, ⌜ w = vr.[ρ] ⌝) ⊢@{iPropI Σ}
+    □(⟦ T1 ⟧ ρ v ∗-∗ ⟦ T2 ⟧ ρ v).
   Proof.
     (* V1: gets type error at Qed, due to [dependent induction]. *)
-    (* intros Hrew; move: v ρ; dependent induction Hrew => v ρ; *)
+    intros Hrew; move: v ρ; dependent induction Hrew => v ρ;
     (* V2 *)
-    move HE: (pv vr) => q; move => Hrew; move: v ρ vr HE. induction Hrew => v ρ vr HE; subst q;
-      last apply rewrite_tsel_psubst2; iIntros "/= #H !>"; iSplit.
+    (* move HE: (pv vr) => q; move => Hrew; move: v ρ vr HE. induction Hrew => v ρ vr HE; subst q; *)
+      last apply skip; iIntros "/= #H !>"; iSplit.
     1-4: iIntros "[??]"; iFrame; by iApply IHHrew.
     1-4: iIntros "[?|?]"; iFrame; by (iLeft + iRight); iApply IHHrew.
     1-2: iIntros "? !>"; by iApply IHHrew.
@@ -428,17 +551,6 @@ Section foo.
 
   rewrite decide_False; simplify_eq/=. done. naive_solver. congruence. *)
 
-  (* Special cases, any use? *)
-  Lemma path_replacement_equiv_plain_special {p vr ρ} q (φ : vl → iProp Σ):
-    path_wp p.|[ρ] (λ w, ⌜ w = vr.[ρ] ⌝) ⊢@{iPropI Σ}
-    path_wp q.|[ρ] φ ≡ path_wp (q .p[p := pv vr]).|[ρ] φ.
-  Proof. by rewrite -path_replacement_equiv_plain -simpl_alias_1. Qed.
-
-  Lemma rewrite_tsel_psubst2_special p q l ρ v vr:
-    path_wp p.|[ρ] (λ w, ⌜ w = vr.[ρ] ⌝) ⊢@{iPropI Σ}
-    ⟦ TSel q l ⟧ ρ v ≡ ⟦ TSel (q .p[ p := pv vr ]) l ⟧ ρ v.
-  Proof. exact: path_replacement_equiv_plain_special. Qed.
-
   (* Lemma path_replacement p q vr ρ φ:
     □path_wp p.|[ρ] (λ w, ⌜ w = vr.[ρ] ⌝) ⊢@{iPropI Σ}
     □(path_wp q.|[ρ] φ -∗ path_wp (q .p[p := pv vr]).|[ρ] φ).
@@ -456,4 +568,4 @@ Section foo.
     iApply (path_replacement_equiv with "Heq HA").
   Qed. *)
 
-End foo.
+End path_repl.
